Introducing no_auto_projectors_decls attribute
The no_auto_projector attribute prevents F* from generating
*definitions* for the projectors, but the type declarations
and SMT encoding are still there. This attribute prevents F* from
generating anything about projectors.

Discriminators are still generated.

ulib/FStar.Pervasives.fst
@@ -188,6 +188,8 @@ let strictly_positive = ()
 
 let unused = ()
 
+let no_auto_projectors_decls = ()
+
 let no_auto_projectors = ()
 
 let no_subtyping = ()
