ulib/FStar.Pervasives.fsti
@@ -1177,6 +1177,7 @@ val unused : unit
     typechecking lot of projectors, most of which are not going to be used
     in the rest of the program
   *)
+val no_auto_projectors_decls : unit
 val no_auto_projectors : unit
 
 (** This attribute can be added to a let definition
